code/ecdsap256/CHANGES.md
@@ -1,0 +1,6 @@
+## Modifications
+
+### 25.03.2022
+
+- Added CHANGES.md file
+- Modified the multiplicaion to use the existing one
